frickin finally

crash_safe_disk.dfy
@@ -1,60 +1,179 @@
-abstract module Synchronous_Disk {
-  type LBA(==)
-  type Datum
+include "map_utils.dfy"
+  
+module Logging_int_int_Map /* refines Crash_Safe_Data_Structure */ {
+  import Map_Utils
 
-  // We model a disk as a mutable map from LBAs to Datums
-  type State = map<LBA, Datum>
+  type LBA = int
+  type Datum = (int, int)
+  type Disk = map<LBA, Datum>
     
-  trait Disk {
-    function Interpret() : map<LBA, Datum>
-      
-    method Read(lba: LBA) returns (result: Datum)
-      requires lba in Interpret();
-      ensures result == Interpret()[lba];
+  type StructureInterpretation = map<int, int>
 
-    method Write(lba: LBA, datum: Datum)
-      ensures Interpret() == old(Interpret())[lba := datum];
+  predicate Valid(disk: Disk)
+  {
+    0 in disk &&
+      disk[0].0 >= 0 &&
+      disk[0].1 == 0 &&
+      (forall i :: 1 <= i <= disk[0].0 ==> i in disk)
   }
-}
 
-// A crash-safe disk enforces that every write either
-// - not change the post-crash state, or
-// - ensure that the post-crash state is the current state
-abstract module Crash_Safe_Disk refines Synchronous_Disk {
-  import DS: On_Disk_Data_Structure
-
-  trait Disk {
-    var mem: DS.In_Memory_State
-    ghost var post_crash_mem: DS.In_Memory_State
+  function method LastEntry(disk: Disk) : int
+    requires Valid(disk);
+  {
+    disk[0].0
+  }
       
+  function PostCrashInterpretation(disk: Disk) : StructureInterpretation
+    requires Valid(disk);
+    decreases LastEntry(disk);
+  {
+    if LastEntry(disk) <= 0 then map[]
+    else
+      var lastEntry := LastEntry(disk);
+      var disk' := disk[0 := (lastEntry - 1, 0)];
+      PostCrashInterpretation(disk')[disk[lastEntry].0 := disk[lastEntry].1]
+  }
+
+  function TrimLastLogEntry(disk: Disk) : Disk
+    requires Valid(disk);
+    requires LastEntry(disk) > 0;
+    ensures Valid(TrimLastLogEntry(disk));
+  {
+    disk[0 := (LastEntry(disk)-1, 0)]
+  }
+
+  lemma DiskInterpretationIgnoresExtra(a: Disk, b: Disk)
+    requires Valid(a);
+    requires Valid(b);
+    requires LastEntry(a) == LastEntry(b);
+    requires forall i :: 0 <= i <= LastEntry(a) ==> a[i] == b[i];
+    ensures PostCrashInterpretation(a) == PostCrashInterpretation(b);
+    decreases LastEntry(a);
+  {
+    if LastEntry(a) > 0 {
+      var a' := TrimLastLogEntry(a);
+      var b' := TrimLastLogEntry(b);
+      DiskInterpretationIgnoresExtra(a', b');
+    }
+  }
+  
+  type InMemoryState = seq<(int, int)>
+    
+  function TailSeqInterpretation(log: seq<(int, int)>) : StructureInterpretation
+  {
+    if |log| == 0 then map[]
+    else TailSeqInterpretation(log[..|log|-1])[log[|log|-1].0 := log[|log|-1].1]
+  }
+  
+  function OverallInterpretation(disk: Disk, mem: InMemoryState) : StructureInterpretation
+    requires Valid(disk);
+  {
+    var diskmap: StructureInterpretation := PostCrashInterpretation(disk);
+    var memmap: StructureInterpretation := TailSeqInterpretation(mem);
+    Map_Utils.union_preferA(memmap, diskmap)
+  }
+
+  lemma CommittingUpdatesInterpretation(disk: Disk, mem: InMemoryState)
+    requires Valid(disk);
+    requires forall i :: 0 <= i <= disk[0].0 + |mem| ==> i in disk;
+    requires forall i :: 0 <= i < |mem| ==> disk[disk[0].0 + i + 1] == mem[i];
+    ensures Valid(disk[0 := (disk[0].0 + |mem|, 0)]);
+    ensures OverallInterpretation(disk[0 := (LastEntry(disk) + |mem|, 0)], []) ==
+      OverallInterpretation(disk, mem);
+    decreases |mem|;
+  {
+    if |mem| == 0 {
+      var disk' := disk[0 := (LastEntry(disk) + |mem|, 0)];
+      assert disk' == disk; // Observe
+    } else if |mem| == 1 {
+      var k := mem[0].0;
+      var v := mem[0].1;
+      var disk' := disk[0 := (LastEntry(disk) + |mem|, 0)];
+      assert disk'[0 := (disk'[0].0 - 1, 0)] == disk; // Observe
+    } else {
+      CommittingUpdatesInterpretation(disk, mem[0..|mem|-1]);
+      var disk' := disk[0 := (LastEntry(disk) + |mem|-1, 0)];
+      CommittingUpdatesInterpretation(disk', mem[|mem|-1..|mem|]);
+      var disk'' := disk'[0 := (LastEntry(disk') + 1, 0)];
+      assert disk'' == disk[0 := (LastEntry(disk) + |mem|, 0)]; // Observe
+    }
+  }
+  
+  class Logging_int_int_Map {
+    var disk: Disk
+    var mem: InMemoryState
+
+    method Set(k: int, v: int)
+      requires Valid(disk);
+      ensures Valid(disk);
+      ensures OverallInterpretation(disk, mem) == old(OverallInterpretation(disk, mem))[k := v];
+      modifies this;
+    {
+      mem := mem + [(k, v)];
+    }
+
+    method MakeDurable()
+      requires Valid(disk);
+      ensures Valid(disk);
+      ensures PostCrashInterpretation(disk) == OverallInterpretation(disk, mem);
+      ensures OverallInterpretation(disk, mem) == old(OverallInterpretation(disk, mem));
+      modifies this;
+    {
+      if |mem| > 0 {
+        var i := 0;
+        while i < |mem|
+          invariant 0 <= i <= |mem|;
+          invariant Valid(disk);
+          invariant |mem| > 0;
+          invariant forall j :: LastEntry(disk) + 1 <= j < LastEntry(disk) + 1 + i ==> j in disk;
+          invariant forall j :: 0 <= j < i ==> disk[LastEntry(disk) + j + 1] == mem[j];
+          invariant OverallInterpretation(disk, mem) == old(OverallInterpretation(disk, mem));
+          invariant PostCrashInterpretation(disk) == old(PostCrashInterpretation(disk));
+        {
+          Write(LastEntry(disk) + i + 1, mem[i]);
+          i := i + 1;
+        }
+        CommittingWrite(0, (LastEntry(disk) + |mem|, 0));
+      }
+    }
+    
+    method Read(lba: LBA) returns (result: Datum)
+      requires Valid(disk);
+      requires lba in disk;
+      ensures result == disk[lba];
+    {
+      result := disk[lba];
+    }
+
     method Write(lba: LBA, datum: Datum)
-      ensures Interpret() == old(Interpret())[lba := datum];
-      ensures DS.Interpret(post_crash_mem, Interpret()) == DS.Interpret(post_crash_mem, old(Interpret()));
+      requires Valid(disk);
+      requires lba > LastEntry(disk);
+      ensures Valid(disk);
+      ensures disk == old(disk)[lba := datum];
+      ensures PostCrashInterpretation(disk) == old(PostCrashInterpretation(disk));
+      ensures mem == old(mem);
+      modifies this;
+    {
+      DiskInterpretationIgnoresExtra(disk, disk[lba := datum]);
+      disk := disk[lba := datum];
+    }
 
     method CommittingWrite(lba: LBA, datum: Datum)
-      ensures Interpret() == old(Interpret())[lba := datum];
-      ensures DS.Interpret(post_crash_mem, Interpret()) == DS.Interpret(mem, old(Interpret()));
-
-    constructor()
+      requires Valid(disk);
+      requires |mem| > 0;
+      requires lba == 0;
+      requires datum == (LastEntry(disk) + |mem|, 0);
+      requires forall i :: 0 <= i <= datum.0 ==> i in disk;
+      requires forall i :: 0 <= i < |mem| ==> disk[LastEntry(disk) + 1 + i] == mem[i];
+      ensures Valid(disk);
+      ensures disk == old(disk)[lba := datum];
+      ensures PostCrashInterpretation(disk) == old(OverallInterpretation(disk, mem));
+      ensures OverallInterpretation(disk, mem) == old(OverallInterpretation(disk, mem));
+      modifies this;
+    {
+      CommittingUpdatesInterpretation(disk, mem);
+      disk := disk[lba := datum];
+      mem := [];
+    }
   }
 }
-
-abstract module On_Disk_Data_Structure {
-  import Disk_Model: Synchronous_Disk
-    
-  type Interpretation(==)
-
-  class In_Memory_State {
-    constructor()
-  }
-
-  function Interpret(mem: In_Memory_State, disk: map<Disk_Model.LBA, Disk_Model.Datum>) : Interpretation
-  
-}
-
-  
-abstract module Crash_Safe_Data_Structure refines On_Disk_Data_Structure {
-  import Disk_Model = Crash_Safe_Disk
-    
-}
-  
